%!TEX root = focs.tex


\section{Off}
\begin{mylem}
	Let $\bs$ a $\beta$ stationary strategies, then $\bs$ is a $\beta $discounted stationary equilibrium if and only if for every $q$ such that $\pr^{\bs}(q \mid q_0) \neq 0$ and every strategy $s'_p$ we have $u_p(\bs \mid q) \geq u_p((\bs_{-p},s'_p) \mid q)$.
\end{mylem}
\begin{proof}
	Especially $\pr^{\bs}(q_0 \mid q_0) = 1$ therefore for every strategy $s'_p$ we have $u_p(\bs \mid q_0) \geq u_p((\bs_{-p},s'_p) \mid q_0)$ so $\bs$ is a $\beta $discounted stationary equilibrium.
	
	Suppose that $\bs$ is a $\beta$ discounted stationary equilibrium and exists $q$ such that $\pr^{\bs}(q \mid q_0) \neq 0$ and a strategy $s'_p$ for which $u_p(\bs \mid q) < u_p((\bs_{-p},s'_p) \mid q)$.
	Then we build the strategy $s''_p$ such that for each $q'$ if $\pr^{(\bs_{-p},s'_p)}(q' \mid q) \neq 0$ then $s''_p(q') = s'_p(q')$ and $s''_p(q') = s_p(q')$ otherwise. Clearly we have that $u_p(\bs \mid q_0) < u_p((\bs_{-p},s''_p) \mid q_0)$ therefore $\bs$ is not a $\beta$ discounted stationary equilibrium.
\end{proof}

The definition of $meet(q,p)$ has disappear from the paper here is mine :  
$$\meet(q,p)  =  {\displaystyle \max_{\preceq} \ \{b \in meet(q) \mid  \text{for every } b' \in \longest(q,p): b \preceq b'\}}$$

For any $q$ body knowledge we denote
$meet(q,\bP)$ the value $$\meet(q,\bP)  =  {\displaystyle \max_{\preceq} \ \{b \in meet(q) \mid \text{for every } p\in \bP \text{ and for every } b' \in \longest(q,p): b \preceq b'\}}$$

\begin{mylem}
	\label{lem-meet}
	Let $\bs$ greedy stationary strategies. for every pair $q$ and $q'$ of bodies of knowledge such that $\pr^{\bs'}(q' \mid q) \neq 0$ then $meet(q,\bP) \preceq meet(q')$
\end{mylem}	
\begin{proof}
	By induction : 
	\\Clearly we have $meet(q,\bP) \preceq meet(q)$.
	\\Assume $q'$ a body of knowledge such that $\pr^{\bs'}(q' \mid q) \neq 0$ and $meet(q,\bP) \preceq meet(q')$. So we also have that $meet(q,\bP) \preceq meet(q',\bP)$. Moreover $\bs$ is a greedy stationary strategies so $meet(q',\bP) \preceq meet(s_p(q')(q'),\bP)$. Hence $meet(q,\bP) \preceq meet(s_p(q')(q'),\bP)$.
	
\end{proof}

\begin{mylem}
	Let $\bs$ a strategies we have  
	\begin{eqnarray*}
		u_p^n(\bs \mid q) & = & u_p^k(\bs \mid q) + \sum_{q' \in \bQ \,:\, q \subseteq q'}^{|q'| = |q|+k} \beta^{|q|+k} \cdot  u_p^{n-k}(\bs \mid q') \cdot \pr^{\bs}(q' \mid q) \\
	 \end{eqnarray*}
\end{mylem}
\begin{proof}
	A bit of math i hope it is working (it should)
\end{proof}

\begin{mylem}
	Let $\bs = (s_1,s_2)$ be a $\beta$ discounted stationary equilibrium in an infinite mining game with two players. 
	Then the combined strategy $\bs'$ such that for any player $p$  and for every $q$ body of knowledge such that $\subbody(q,\meet(q,p)) = q$ then $s'_p(q) = s_p(q)$,
	and for every pair $q$ and $q'$ of 
	bodies of knowledge in which $\subbody(q,\meet(q,p)) = \subbody(q',\meet(q',p))$ we have that 
	$s'_p(q) = s'_p(q')$ is a $\beta$ discounted stationary equilibrium and $u_p(\bs \mid q_0) = u_p(\bs' \mid q_0)$
\end{mylem}
\etienne{While formally writing the proof we have some maybe useless but pretty properties over the s' we can build, if s doesnt "directly satisfies" the lemma then s' can be construct using any of the action over all the "equivalent" state, i dont really know how to formally write that down but it is fun. This property also implies that if we are able to show that there exits a dominant strategy for any p over the base cases then there exists also a unique equilibrium over the full game.} 

\begin{proof} 
	
\begin{mylem}
	\label{lemrew}
	For any player $p$ and any body of knowledge $q$ we have $r_p(s_p(q)(q)) =r_p(s'_p(q)(q))$ and $r_p(s_{1-p}(q)(q)) =r_p(s'_{1-p}(q)(q))$
\end{mylem}
\begin{proof}
	\iffalse	By induction :
	
	As for any $p$, $s_p(q_0) = s'_p(q_0)$ we have $r_p(s_p(q_0)(q_0)) =r_p(s'_p(q_0)(q_0))$ and $r_p(s_{1-p}(q_0)(q_0)) =r_p(s'_{1-p}(q_0)(q_0))$.
	
	Suppose that there exists $n$ such that for any $q$ with $|q| \leq n$ then $r_p(s_p(q)(q)) =r_p(s'_p(q)(q))$ and $r_p(s_{1-p}(q)(q)) =r_p(s'_{1-p}(q)(q))$
	\fi
	
	Let $a$ a greedy action then
	\begin{eqnarray*}
		r_p(a(q)) &= & {\displaystyle c \cdot \sum_{i=1}^{|\meet(a(q))|} \alpha^i \cdot \chi_p(\meet(a(q)),i)} \ \\
		r_p(a(q)) &= & {\displaystyle c \cdot \sum_{i=1}^{|\meet(q,\bP)|} \alpha^i \cdot \chi_p(\meet(q,\bP),i)} \ \\
		&&+ {\displaystyle c \cdot \sum_{i=|\meet(q,\bP)|+1}^{|\meet(a(q))|} \alpha^i \cdot \chi_p(meet(a(q)),i)} \ \\
		r_p(a(q)) &= & r_p(\meet(q,\bP)) \ \\
		&&+ \alpha^{|\meet(q,\bP)|} \cdot {\displaystyle c \cdot \sum_{i=1}^{|meet(\subbody(a(q),\meet(q,\bP)))|} \alpha^i \cdot \chi_p(meet(\subbody(a(q),\meet(q,\bP))),i)} \ \\
		r_p(a(q)) &= & r_p(\meet(q,\bP)) + \alpha^{|\meet(q,\bP)|} \cdot r_p(\subbody(a(q),\meet(q,\bP))) \\
	\end{eqnarray*}

	\begin{mylem}
		\begin{eqnarray*}
		\subbody(s'_p(q)(q),\meet(q,\bP)) & = & s'_p(\subbody(q,\meet(q,\bP)))(\subbody(q,\meet(q,\bP))) \\
		\subbody(s'_{1-p}(q)(q),\meet(q,\bP)) & = & s'_{1-p}(\subbody(q,\meet(q,\bP)))(\subbody(q,\meet(q,\bP))) \\
		\end{eqnarray*}
	\end{mylem}
\begin{proof}
	Trivial by def of s'
\end{proof}

Therefore we have :
\begin{eqnarray*}
	r_p(s'_p(q)(q)) &= & r_p(\meet(q,\bP)) + \alpha^{|\meet(q,\bP)|} \cdot r_p(s'_p(\subbody(q,\meet(q,\bP)))(\subbody(q,\meet(q,\bP)))) \\
	r_p(s'_p(q)(q)) &= & r_p(\meet(q,\bP)) + \alpha^{|\meet(q,\bP)|} \cdot r_p(s_p(\subbody(q,\meet(q,\bP)))(\subbody(q,\meet(q,\bP)))) \\
\end{eqnarray*}

\begin{mylem}
	\begin{eqnarray*}
	r_p(s_p(\subbody(q,\meet(q,\bP)))(\subbody(q,\meet(q,\bP)))) &=& r_p(\subbody(s_p(q)(q),\meet(q,\bP)))\\
	r_p(s_{1-p}(\subbody(q,\meet(q,\bP)))(\subbody(q,\meet(q,\bP)))) &=& r_p(\subbody(s_{1-p}(q)(q),\meet(q,\bP)))\\
\end{eqnarray*}
\end{mylem}
\begin{proof}
	Notice that for any $q$, $r_p(q) + r_{1-p}(q) = C \cdot |meet(q)|$, therefore we only have to demonstrate that $r_p(s_p(\subbody(q,\meet(q,\bP)))(\subbody(q,\meet(q,\bP)))) = r_p(\subbody(s_p(q)(q),\meet(q,\bP)))$.
	
	If exists $q$ such that $r_p(s_p(\subbody(q,\meet(q,\bP)))(\subbody(q,\meet(q,\bP)))) > r_p(\subbody(s_p(q)(q),\meet(q,\bP)))$ ,
	consider $s''_p$ such that for any $q' \neq q$, $s''_p(q') = s_p(q)$  and $s''_p(q) = s_p(\subbody(q,\meet(q,\bP))$.
	

	\begin{eqnarray*}
		u_p(\bs \mid \subbody(q,\meet(q,\bP)) & = & u_p^{|q|-|\subbody(q,\meet(q,\bP)|}(\bs \mid \subbody(q,\meet(q,\bP)) \\
		&& + \beta^{|q|} \cdot \sum_{q' \in \bQ \,:\, q_0 \subseteq q}^{|q'| = |q|} u_p(\bs \mid q') \cdot \pr^{\bs}(q' \mid \subbody(q,\meet(q,\bP)) \\ 
	\end{eqnarray*}
	\begin{eqnarray*}
		u_p((\bs_{-p},s''_p) \mid \subbody(q,\meet(q,\bP)) & = & u_p^{|q|-|\subbody(q,\meet(q,\bP)|}((\bs_{-p},s''_p) \mid \subbody(q,\meet(q,\bP)) \\
		&& + \beta^{|q|} \cdot \sum_{q' \in \bQ \,:\, q_0 \subseteq q}^{|q'| = |q|} u_p((\bs_{-p},s''_p) \mid q') \cdot \pr^{(\bs_{-p},s''_p)}(q' \mid \subbody(q,\meet(q,\bP)) \\ 
	\end{eqnarray*}
\begin{eqnarray*}
	u_p(\bs \mid \subbody(q,\meet(q,\bP)) - u_p((\bs_{-p},s''_p) \mid \subbody(q,\meet(q,\bP)) & = & u_p(\bs \mid q)- u_p((\bs_{-p},s''_p)  \mid q)\\
\end{eqnarray*}
\end{proof}
	
	Finnaly we have :
	\begin{eqnarray*}
		r_p(s'_p(q)(q)) &= & r_p(\meet(q,\bP)) + \alpha^{|\meet(q,\bP)|} \cdot r_p(s_p(\subbody(q,\meet(q,\bP)))) \\
		r_p(s'_p(q)(q)) &= & r_p(s_p(q)(q))
	\end{eqnarray*}
Similarly we have $r_p(s'_{1-p}(q)(q)) =  r_p(s_{1-p}(q)(q))$
\end{proof}

By induction we show that for any $q$ and for any $s''_p$ we have $u_p( (\bs_{-p},s''_p) \mid q) = u_p( (\bs'_{-p},s''_p) \mid q)$.

\begin{eqnarray*}
	u_p^{1}( (\bs_{-p},s''_p) \mid q) & = & \sum_{q' \in \bQ \,:\, q \subseteq q'}^{|q'| \leq |q|+1} \beta^{|q'|} \cdot  r_p(q') \cdot \pr^{(\bs_{-p},s''_p)}(q' \mid q) \\ 
	& = &  \beta^{|q|} \cdot  r_p(q) + \sum_{q' \in \bQ \,:\, q \subseteq q'}^{|q'| = |q|+1} \beta^{|q'|} \cdot  r_p(q') \cdot \pr^{(\bs_{-p},s''_p)}(q' \mid q)\\ 
	& = & \beta^{|q|} \cdot  r_p(q) + \beta^{|q|+1} \cdot  r_p(s''_p(q)(q)) \cdot h_p + \beta^{|q|+1} \cdot  r_p(s_{1-p}(q)(q)) \cdot h_{1-p}\\
	& = & \beta^{|q|} \cdot  r_p(q) + \beta^{|q|+1} \cdot  r_p(s''_p(q)(q)) \cdot h_p + \beta^{|q|+1} \cdot  r_p(s'_{1-p}(q)(q)) \cdot h_{1-p} \textit{ by lemma \ref{lemrew}}  \\
	& = & u_p^{1}( (\bs'_{-p},s''_p) \mid q)
\end{eqnarray*}
Suppose there exists $N$ such that for any $n \leq N$ and $q$ we have $u_p^n( (\bs_{-p},s''_p) \mid q) = u_p^n( (\bs'_{-p},s''_p) \mid q)$.
\begin{eqnarray*}
	u_p^{n+1}( (\bs_{-p},s''_p) \mid q) & = & u_p^1((\bs_{-p},s''_p) \mid q) + \sum_{q' \in \bQ \,:\, q \subseteq q'}^{|q'| = |q|+1} \beta^{|q|+1} \cdot  u_p^{n}((\bs_{-p},s''_p) \mid q') \cdot \pr^{(\bs_{-p},s''_p)}(q' \mid q) \\
	u_p^{n+1}( (\bs_{-p},s''_p) \mid q) & = & u_p^1((\bs_{-p},s''_p) \mid q) \\
	&& +  \beta^{|q|+1} \cdot  u_p^{n}((\bs_{-p},s''_p) \mid s''_p(q)(q)) \cdot h_p \\
	&&+ \beta^{|q|+1} \cdot  u_p^{n}((\bs_{-p},s''_p) \mid s_{1-p}(q)(q)) \cdot h_{1-p} \\
	u_p^{n+1}( (\bs_{-p},s''_p) \mid q) & = & u_p^1((\bs'_{-p},s''_p) \mid q) \\
	&& +  \beta^{|q|+1} \cdot  u_p^{n}((\bs'_{-p},s''_p) \mid s''_p(q)(q)) \cdot h_p \\
	&&+ \beta^{|q|+1} \cdot  u_p^{n}((\bs'_{-p},s''_p) \mid s_{1-p}(q)(q)) \cdot h_{1-p} \\
	u_p^{n+1}( (\bs_{-p},s''_p) \mid q) & = & u_p^{n+1}( (\bs'_{-p},s''_p) \mid q) \\
\end{eqnarray*}




\begin{mylem}
	\label{lemsup}
	Let $\bs, \bs'$ greedy stationary strategies. Then for any player $p$ and for every $q$ body of knowledge we have that :  $$\alpha^{|meet(q,\bP)|} (u_p(\bs \mid q) - u_p(\bs' \mid q))  =  u_p(\bs \mid \subbody(q,meet(q,\bP))) - u_p(\bs' \mid \subbody(q,meet(q,\bP)))$$ 
\end{mylem}

\end{proof}

\iffalse

\begin{mylem}
	Let $\bs$ a $\beta$ stationary strategies, then $\bs$ is a $\beta $discounted stationary equilibrium if and only if for every $q$ such that $\pr^{\bs}(q \mid q_0) \neq 0$ and every strategy $s'_p$ we have $u_p(\bs \mid q) \geq u_p((\bs_{-p},s'_p) \mid q)$.
\end{mylem}
\begin{proof}
	Especially $\pr^{\bs}(q_0 \mid q_0) = 1$ therefore for every strategy $s'_p$ we have $u_p(\bs \mid q_0) \geq u_p((\bs_{-p},s'_p) \mid q_0)$ so $\bs$ is a $\beta $discounted stationary equilibrium.
	
	Suppose that $\bs$ is a $\beta$ discounted stationary equilibrium and exists $q$ such that $\pr^{\bs}(q \mid q_0) \neq 0$ and a strategy $s'_p$ for which $u_p(\bs \mid q) < u_p((\bs_{-p},s'_p) \mid q)$.
	Then we build the strategy $s''_p$ such that for each $q'$ if $\pr^{(\bs_{-p},s'_p)}(q' \mid q) \neq 0$ then $s''_p(q') = s'_p(q')$ and $s''_p(q') = s_p(q')$ otherwise. Clearly we have that $u_p(\bs \mid q_0) < u_p((\bs_{-p},s''_p) \mid q_0)$ therefore $\bs$ is not a $\beta$ discounted stationary equilibrium.
\end{proof}

The definition of $meet(q,p)$ has disappear from the paper here is mine :  
$$\meet(q,p)  =  {\displaystyle \max_{\preceq} \ \{b \in meet(q) \mid  \text{for every } b' \in \longest(q,p): b \preceq b'\}}$$

Section under construction, mostly to share my preliminary results with you.

For any $q$ body knowledge we denote
$meet(q,\bP)$ the value $$\meet(q,\bP)  =  {\displaystyle \max_{\preceq} \ \{b \in meet(q) \mid \text{for every } p\in \bP \text{ and for every } b' \in \longest(q,p): b \preceq b'\}}$$



\begin{mylem}
	\label{lem-meet}
	Let $\bs$ greedy stationary strategies. for every pair $q$ and $q'$ of bodies of knowledge such that $\pr^{\bs'}(q' \mid q) \neq 0$ then $meet(q,\bP) \preceq meet(q')$
\end{mylem}	
\begin{proof}
	By induction : 
	\\Clearly we have $meet(q,\bP) \preceq meet(q)$.
	\\Assume $q'$ a body of knowledge such that $\pr^{\bs'}(q' \mid q) \neq 0$ and $meet(q,\bP) \preceq meet(q')$. So we also have that $meet(q,\bP) \preceq meet(q',\bP)$. Moreover $\bs$ is a greedy stationary strategies so $meet(q',\bP) \preceq meet(s_p(q')(q'),\bP)$. Hence $meet(q,\bP) \preceq meet(s_p(q')(q'),\bP)$.
	
\end{proof}

\begin{mylem}
	\label{lemsup}
	Let $\bs, \bs'$ greedy stationary strategies. Then for any player $p$ and for every $q$ body of knowledge we have that :  $$\alpha^{|meet(q,\bP)|} (u_p(\bs \mid q) - u_p(\bs' \mid q))  =  u_p(\bs \mid \subbody(q,meet(q,\bP))) - u_p(\bs' \mid \subbody(q,meet(q,\bP)))$$ 
\end{mylem}

\begin{proof}
	By lemma \ref{lem-meet} we have $meet(q,\bP) \preceq meet(q')$ therefore
	\begin{eqnarray*}
		r_p(q') & = &{\displaystyle c \cdot \sum_{i=1}^{|\meet(q')|} \alpha^i \cdot \chi_p(\meet(q'),i)} \\
		& = & {\displaystyle c \cdot \sum_{i=1}^{|meet(q,\bP)|} \alpha^i \cdot \chi_p(meet(q,\bP),i) } \\
		&&	+ {\displaystyle c \cdot \sum_{i=|meet(q,\bP)|+1}^{|\meet(q')|} \alpha^{i} \cdot \chi_p(\subbody(\meet(q'),meet(q,\bP)),i-(|meet(q,\bP)|+1))  }   \\
	\end{eqnarray*}
	Hence 
	\begin{eqnarray*}
		u_p(\bs \mid q)& = & \sum_{q' \in \bQ \,:\, q \subseteq q} \beta^{|q'|} \cdot  r_p(q') \cdot \pr^{\bs}(q' \mid q) \\ 
		& = & \sum_{q' \in \bQ \,:\, q \subseteq q} \beta^{|q'|} \cdot  [{\displaystyle c \cdot \sum_{i=1}^{|meet(q,\bP)|} \alpha^i \cdot \chi_p(meet(q,\bP),i) }] \cdot \pr^{\bs}(q' \mid q) \\
		&+ & \sum_{q' \in \bQ \,:\, q \subseteq q} \beta^{|q'|} \cdot  [{\displaystyle c \cdot \sum_{i=|meet(q,\bP)|+1}^{|\meet(q')|} \alpha^{i} \cdot \chi_p(\subbody(\meet(q'),meet(q,\bP)),i-|meet(q,\bP)|)  }] \cdot \pr^{\bs}(q' \mid q) \\
	\end{eqnarray*}
	Moreover $$ \sum_{q' \in \bQ \,:\, q \subseteq q \,:\, |q'| =k}  \pr^{\bs}(q' \mid q) = 1$$
	So 
	\begin{eqnarray*}
		u_p(\bs \mid q) & = & \sum_{k = |q|}^{\infty} \beta^{k} \cdot  [{\displaystyle c \cdot \sum_{i=1}^{|meet(q,\bP)|} \alpha^i \cdot \chi_p(meet(q,\bP),i) }] \\
		&+ & \sum_{q' \in \bQ \,:\, q \subseteq q} \beta^{|q'|} \cdot  [{\displaystyle c \cdot \sum_{i=|meet(q,\bP)|+1}^{|\meet(q')|} \alpha^{i} \cdot \chi_p(\subbody(\meet(q'),meet(q,\bP)),i-|meet(q,\bP)|)  }] \cdot \pr^{\bs}(q' \mid q) \\
	\end{eqnarray*}
	
	Therefore
	\begin{eqnarray*}
		u_p(\bs \mid q) - u_p(\bs' \mid q) & = & [\sum_{k = |q|}^{\infty} \beta^{k} \cdot  [{\displaystyle c \cdot \sum_{i=1}^{|meet(q,\bP)|} \alpha^i \cdot \chi_p(meet(q,\bP),i) }] \\
		&+ & \sum_{q' \in \bQ \,:\, q \subseteq q} \beta^{|q'|} \cdot  [{\displaystyle c \cdot \sum_{i=|meet(q,\bP)|+1}^{|\meet(q')|} \alpha^{i} \cdot \chi_p(\subbody(\meet(q'),meet(q,\bP)),i-|meet(q,\bP)|)  }] \cdot \pr^{\bs}(q' \mid q) ]\\ 
		&- &[\sum_{k = |q|}^{\infty} \beta^{k} \cdot  [{\displaystyle c \cdot \sum_{i=1}^{|meet(q,\bP)|} \alpha^i \cdot \chi_p(meet(q,\bP),i) }] \\
		&+ & \sum_{q' \in \bQ \,:\, q \subseteq q} \beta^{|q'|} \cdot  [{\displaystyle c \cdot \sum_{i=|meet(q,\bP)|+1}^{|\meet(q')|} \alpha^{i} \cdot \chi_p(\subbody(\meet(q'),meet(q,\bP)),i-|meet(q,\bP)|)  }] \cdot \pr^{\bs'}(q' \mid q) ]\\ 
		u_p(\bs \mid q) - u_p(\bs' \mid q) & = & \sum_{q' \in \bQ \,:\, q \subseteq q} \beta^{|q'|} \cdot  [{\displaystyle c \cdot \sum_{i=|meet(q,\bP)|+1}^{|\meet(q')|} \alpha^{i)} \cdot \chi_p(\subbody(\meet(q'),meet(q,\bP)),i-|meet(q,\bP)|)  }] \cdot \pr^{\bs}(q' \mid q) \\ 
		& - & \sum_{q' \in \bQ \,:\, q \subseteq q} \beta^{|q'|} \cdot  [{\displaystyle c \cdot \sum_{i=|meet(q,\bP)|+1}^{|\meet(q')|} \alpha^{i} \cdot \chi_p(\subbody(\meet(q'),meet(q,\bP)),i-|meet(q,\bP)|)  }] \cdot \pr^{\bs'}(q' \mid q) \\
	\end{eqnarray*}
	Clearly we have $|meet(q')| = |meet(q,\bP)| + |\subbody(\meet(q'),\meet(q,\bP))| $ hence 
	\begin{eqnarray*}
		\alpha^{|meet(q,\bP)|} (u_p(\bs \mid q) - u_p(\bs' \mid q)) & = & \sum_{q' \in \bQ \,:\, q \subseteq q} \beta^{|q'|} \cdot  [{\displaystyle c \cdot \sum_{i=1}^{|\subbody(\meet(q'),meet(q,\bP))} \alpha^{i} \cdot \chi_p(\subbody(\meet(q'),meet(q,\bP)),i)  }] \cdot \pr^{\bs}(q' \mid q) \\ 
		& - & \sum_{q' \in \bQ \,:\, q \subseteq q} \beta^{|q'|} \cdot  [{\displaystyle c \cdot \sum_{i=1}^{|\subbody(\meet(q'),meet(q,\bP))} \alpha^{i} \cdot \chi_p(\subbody(\meet(q'),meet(q,\bP)),i)  }] \cdot \pr^{\bs'}(q' \mid q) \\
		\alpha^{|meet(q,\bP)|} (u_p(\bs \mid q) - u_p(\bs' \mid q)) & = & u_p(\bs \mid \subbody(q,meet(q,\bP))) - u_p(\bs' \mid \subbody(q,meet(q,\bP))) \\
	\end{eqnarray*}
\end{proof}
\fi

	

\iffalse
Suppose there exists $n$ such that $u_p^n( (\bs_{-p},s''_p) \mid q_0) = u_p^n( (\bs'_{-p},s''_p) \mid q_0)$. 
\begin{eqnarray*}
	u_p^{n+1}( (\bs_{-p},s''_p) \mid q_0) & = & \sum_{q' \in \bQ \,:\, q \subseteq q}^{|q'| \leq n+1} \beta^{|q'|} \cdot  r_p(q') \cdot \pr^{(\bs_{-p},s''_p)}(q' \mid q) \\ 
	u_p^{n+1}( (\bs_{-p},s''_p) \mid q_0) & = & \sum_{q' \in \bQ \,:\, q \subseteq q}^{|q'| \leq n } \beta^{|q'|} \cdot  r_p(q') \cdot \pr^{(\bs_{-p},s''_p)}(q' \mid q) \\
	&& +   \sum_{q' \in \bQ \,:\, q \subseteq q}^{|q'| = n+1 } \beta^{|q'|} \cdot  r_p(q') \cdot \pr^{(\bs_{-p},s''_p)}(q' \mid q) \\
	u_p^{n+1}( (\bs_{-p},s''_p) \mid q_0) & = & u_p^{n}( (\bs_{-p},s''_p) +   \sum_{q' \in \bQ \,:\, q \subseteq q}^{|q'| = n+1 } \beta^{|q'|} \cdot  r_p(q') \cdot \pr^{(\bs_{-p},s''_p)}(q' \mid q) \\
	u_p^{n+1}( (\bs_{-p},s''_p) \mid q_0) & = & u_p^{n}( (\bs'_{-p},s''_p) +   \sum_{q' \in \bQ \,:\, q \subseteq q}^{|q'| = n+1 } \beta^{|q'|} \cdot  r_p(q') \cdot \pr^{(\bs_{-p},s''_p)}(q' \mid q) \\
\end{eqnarray*}

First notice that if $|longest(q,p)| = |longest(q,1-p)|$ then $meet(q,p) = meet(q,1-p) = meet(q,\bP)$. Moreover if $meet(q,p) \neq meet(q,\bP)$ then $meet(q,p) = longest(q,p) = longest(q)$

Assume that $meet(q,\bP) \neq meet(q,p)$:
\\Then $meet(q,p) = longest(q)$ therefore by definition there is only one available greedy action for player $p$, therefore $s'_p(q) = s_p(q) = mine(p,longest(q),q)$. 

Assume that $meet(q,\bP) = meet(q,p)$,
by absurd assume exists $s''_p$ a strategy for player $p$ such that $u_p ((\bs'_{-p},s''_p) \mid q) > u_p(\bs' \mid q)$.
\\By lemma \ref{lemsup} we have, $u_p((\bs'_{-p},s''_p) \mid \subbody(q,meet(q,\bP))) - u_p(\bs' \mid \subbody(q,meet(q,\bP))) > 0$. 
\\As $\subbody(q,meet(q,\bP)) = \subbody(\subbody(q,meet(q,\bP)),\meet(\subbody(q,meet(q,\bP)),p))$ and by definition of $\bs'$ we have $s'_p(\subbody(q,\meet(q,p)) = s_p(\subbody(q,\meet(q,p))$. Hence $u_p((\bs'_{-p},s''_p) \mid \subbody(q,\meet(q,p))) > u_p(\bs \mid \subbody(q,\meet(q,p)))$ therefore $\bs$ is not a $\beta$ discounted stationary equilibrium, which is absurd.

\begin{mylem}
	Let $\bs = (s_1,s_2)$ be a $\beta$ discounted stationary equilibrium in an infinite mining game with two players.  And $\bs' = (s'_1,s'_2)$ greedy strategies. Such that for any $p$, 
	$u_p((s'_1,s_2) \mid q_0) = u_p((s_1,s_2) \mid q_0)$ and $u_p((s_1,s'_2) \mid q_0) = u_p((s_1,s_2) \mid q_0)$ then $\bs'$ is a $\beta$ discounted stationary equilibrium and for any $p$, $u_p(\bs \mid q_0) = u_p(\bs' \mid q_0)$.
\end{mylem}
\begin{proof}
	By absurd assume exists $s''_1$ a strategy  such that $u_1((s''_1,s'_2) \mid q_0) > u_1((s'_1,s'_2) \mid q_0)$. As $\bs$ is a  $\beta$ discounted stationary equilibrium, we have $u_1((s_1,s_2)\mid q_0) \geq u_1((s''_1,s_2)\mid q_0)$. Moreover over as $u_1((s_1,s_2)\mid q_0) = u_1((s_1,s'_2)\mid q_0)$ we have, $u_1((s_1,s'_2)\mid q_0) \geq u_1((s''_1,s_2)\mid q_0)$
\end{proof}
\fi
\iffalse
\etienne{What i am currently working on : }
\begin{myprop}
	Let $\bs = (s_1,s_2)$ a $\beta$ discounted nash equilibrium then $\bs$ is greedy.
\end{myprop}
\begin{proof}
	Let $q$ a state. Let $L \in q$ a list. We denote by $\#(p1,L)$ the number of block own by $p1$ in $L$. Notice that  $\#(p1,L) + \#(p2,L) = |L|$.
	
	By absurd, let $q$ a state such that $s_1(q) = L$ and exists a state $q'$ such that $s_1(q)(q) \subseteq q'$ and $|s_1(q')| < |L|$.
	Let $q'$ one of the first, hence a element such that for all $q''$ , $q'' \subseteq q'$ implies that $s_1(q'') \geq |L|$ .
	
	Hence we have that $\#(p_1, L' \cap q) = \#(p_1, L')$
	\begin{itemize}
		\item suppose that $\#(p_1, L') \geq \#(p_1, L)$ 
		\item suppose that $\#(p_1, L') > \#(p_1, L)$ 
			Then $\#(p_2, L') \leq \#(p_2, L)$
		So $p_2$ will not mine on it, and i exclude it too (next step of the proof)
	\end{itemize}

	\begin{mylem}
		Let $s_1,s_2$ a pair of strategy.
		Let $q$ a state such that $s_1(q) = L$ and exists $L' \in q$ such that $\#(p_1, L') \geq \#(p_1, L)$ and $|L'| \geq |L|$ then exists $s$ such that $u_1((s,s_2),q_0) > u_1((s_1,s_2),q_0)$
	\end{mylem}
\end{proof}
\fi




